typechecks but lots admitted

Instances/Galois.v
@@ -16,18 +16,17 @@ Require Import Types.Result.
 Require Import Types.State.
 Require Import Types.Stores.
 
-Inductive gamma_par : parity -> nat -> Prop :=
-  | gamma_par_even : forall n, even n -> gamma_par par_even n
-  | gamma_par_odd  : forall n, odd n -> gamma_par par_odd n
-  | gamma_par_top : forall n, gamma_par par_top n.
-Hint Constructors gamma_par : soundness.
+Definition gamma_par (p : parity) (n : nat) : Prop :=
+  match p with
+  | par_even => Nat.Even n
+  | par_odd => Nat.Odd n
+  | par_top => True
+  | par_false => False
+  end. 
+Hint Unfold gamma_par : soundness.
 
-Lemma gamma_par_monotone : forall p1 p2,
-  preorder p1 p2 -> preorder (gamma_par p1) (gamma_par p2).
-Proof.
-  destruct p1, p2; simpl; intros; try constructor; try inversion H;
-  intros; try tauto; constructor; inversion H0.
-Qed.
+Lemma gamma_par_monotone : monotone gamma_par.
+Proof. simple_solve. Qed.
 
 Instance galois_parity_nat : Galois nat parity :=
 {
@@ -35,54 +34,12 @@ Instance galois_parity_nat : Galois nat parity :=
   gamma_monotone := gamma_par_monotone;
 }.
 
-Lemma extract_S_n : forall n,
-  extract_par (S n) = parity_plus (extract_par n) par_odd.
-Proof.
-  intros. induction n.
-  - reflexivity.
-  - rewrite -> IHn. simpl. rewrite -> parity_plus_assoc. simpl.
-    rewrite <- parity_plus_par_even. reflexivity.
-Qed.
-
-Lemma even_extract_pareven : forall n,
-  even n -> extract_par n = par_even.
-Proof. 
-  intros. 
-  apply even_equiv in H. destruct H as [k H]; subst.
-  induction k.
-  - (*  0 *)
-    reflexivity.
-  - (* S x *)
-    replace (2 * S k) with (S (S (2 * k))).
-    + repeat rewrite extract_S_n. rewrite IHk. reflexivity.
-    + ring.
-Qed.
-
-Lemma odd_extract_parodd : forall n, odd n -> extract_par n = par_odd.
-Proof. 
-  intros. apply odd_equiv in H. destruct H as [k H]; subst.
-  induction k.
-  - reflexivity.
-  - replace (2 * (S k) + 1) with (S(2 * (S k))).
-    rewrite extract_S_n. replace (2 * S k) with  (S ((2 * k + 1))).
-    rewrite extract_S_n. rewrite IHk. reflexivity. ring. ring.
-Qed.
-
-
-Inductive gamma_interval : interval -> nat -> Prop :=
-  | gamma_interval_in_range : 
-      forall i n, preorder (min i) n  -> 
-                  preorder n (max i) -> 
-                  gamma_interval i n.
-Hint Constructors gamma_interval : soundness.
+Definition gamma_interval (i : interval) (n : nat) : Prop :=
+  preorder (min i) n /\ preorder n (max i).
+Hint Unfold gamma_interval : soundness.
 
 Lemma gamma_interval_monotone : monotone gamma_interval.
-Proof. 
-  intros i i' Hi. constructor. intros n Hn. 
-  constructor; destruct Hn; destruct Hi.
-  apply preorder_trans with (y:=min i); assumption.
-  apply preorder_trans with (y:=max i); assumption.
-Qed.
+Proof. simple_solve. Qed.
 
 Instance  galois_interval : Galois nat interval :=
 {
@@ -90,18 +47,18 @@ Instance  galois_interval : Galois nat interval :=
   gamma_monotone := gamma_interval_monotone;
 }.
 
-Inductive gamma_bool : abstr_bool -> bool -> Prop :=
-  | gamma_true : gamma_bool ab_true true
-  | gamma_false : gamma_bool ab_false false
-  | gamma_ab_top : forall b, gamma_bool ab_top b.
-Hint Constructors gamma_bool : soundness.
+Definition gamma_bool (a : abstr_bool) (b : bool) : Prop :=
+  match a, b with
+  | ab_true, true
+  | ab_false, false
+  | ab_top, _ => True
+  | _, _ => False
+  end.
+Hint Unfold gamma_bool : soundness.
 
 Lemma gamma_bool_monotone : monotone gamma_bool.
 Proof.
-  constructor. intros b Hgamma. destruct b. inversion Hgamma; subst.
-  inversion H; constructor.
-  inversion H; constructor. 
-  inversion H; subst; inversion Hgamma; constructor.
+  simple_solve.
 Qed.
 
 Instance galois_boolean : Galois bool abstr_bool :=
@@ -114,18 +71,15 @@ Section galois_functions.
 Context {A A' B B' : Type} 
   `{Galois B A, Galois B' A'}.
 
-Inductive gamma_fun : (A-> A') -> (B -> B') -> Prop :=
-  | gamma_fun_increasing : forall (f : A -> A') (f' : B -> B'),
-    (forall (a : A) (b : B), gamma a b -> gamma (f a) (f' b)) -> 
-    gamma_fun f f'.
+Definition gamma_fun (f : A -> A') (g : B -> B') : Prop :=
+  forall a b, gamma a b -> gamma (f a) (g b).
+Hint Unfold gamma_fun : soundness. 
 
 Lemma gamma_fun_monotone :
   monotone gamma_fun.
 Proof.
-  constructor.
-  intros x Hgamma. inversion H3; subst. constructor. intros.
-  apply widen with (f:= a a0). apply H4. destruct Hgamma.
-  apply H6. apply H5.
+  simple_solve.
+  apply widen with (f:= a a0). apply H3. auto.
 Qed.
 
 Global Instance GFun : 
@@ -136,25 +90,23 @@ Global Instance GFun :
 }.
 
 End galois_functions.
-Hint Constructors gamma_fun : soundness.
+Hint Unfold gamma_fun : soundness.
 
 Section galois_values.
 
-Inductive gamma_value : avalue -> cvalue -> Prop :=
-  | gamma_value_parity : forall p n,
-      gamma p n -> gamma_value (VParity p) (VNat n)
-  | gamma_value_interval : forall i n,
-      gamma i n -> gamma_value (VInterval i) (VNat n)
-  | gamma_value_bool : forall ab b,
-      gamma ab b -> gamma_value (VAbstrBool ab) (VBool b)
-  | gamma_value_top : forall v, gamma_value VTop v.
-
+Definition gamma_value (a : avalue) (c : cvalue) : Prop :=
+  match a, c with
+  | VParity p, VNat n => gamma p n
+  | VInterval i, VNat n => gamma i n
+  | VAbstrBool ab, VBool b => gamma ab b
+  | VTop, _ => True
+  | _, _ => False
+  end.
+Hint Unfold gamma_value : soundness.
 
 Lemma gamma_value_monotone : monotone gamma_value.
 Proof.
-  constructor. intros x Hgamma. inversion Hgamma; subst;
-   destruct a'; inversion H; subst; try constructor; try assumption;
-    eapply widen; try apply H3; try apply H0.
+  simple_solve. 
 Qed.
 
 Global Instance galois_values : Galois cvalue avalue := 
@@ -163,18 +115,17 @@ Global Instance galois_values : Galois cvalue avalue :=
   gamma_monotone := gamma_value_monotone;
 }.
 End galois_values.
-Hint Constructors gamma_value : soundness.
+Hint Unfold gamma_value : soundness.
 
-
-Inductive gamma_store : abstract_store -> store -> Prop :=
-  | gamma_store_cons : forall st st',
-      (forall x, gamma (st' x) (st x)) -> gamma_store st' st.
-Hint Constructors gamma_store : soundness.
+Definition gamma_store (st' : abstract_store) (st : store) : Prop :=
+  forall x, gamma (st' x) (st x).
+Hint Unfold gamma_store : soundness.
 
 Lemma gamma_store_monotone : monotone gamma_store.
-Proof. constructor. intros st Hgamma.
-  inversion H; subst. constructor. intros x'. inversion Hgamma; subst.
-  apply widen with (f:=a x'); auto.
+Proof. unfold monotone. intros ast ast' H. simpl in *.
+  unfold pointwise_ordering, preordered_set_le in *. intros st Hgamma.
+  unfold gamma_store in *. intro x. eapply widen.
+  apply H. apply Hgamma.
 Qed.
 
 Global Instance galois_store : Galois store abstract_store :=
@@ -186,21 +137,14 @@ Global Instance galois_store : Galois store abstract_store :=
 Section galois_pairs.
 Context {A B C D} `{Galois B A} `{Galois D C}.
 
-Inductive gamma_pairs :
-  prod A C-> prod B D -> Prop := 
-  | gamma_pairs_cons : forall a b c d,
-      gamma a b ->
-      gamma c d ->
-      gamma_pairs (a,c) (b,d).
+Definition gamma_pairs (p : prod A C) (q : prod B D) : Prop :=
+  let (a, c) := p in let (b, d) := q in gamma a b /\ gamma c d.
+Hint Unfold gamma_pairs : soundness.
 
 Lemma gamma_pairs_monotone :
   monotone gamma_pairs.
 Proof.
-  constructor. intros [b d] Hgamma. 
-  destruct H3 as [a a' c c' Haa' Hcc'].
-  inv Hgamma. constructor. 
-  - apply widen with (f:=a); auto. 
-  - apply widen with (f:=c); auto.
+  simple_solve; apply_widen.
 Qed.
 
 Global Instance galois_pairs :
@@ -210,116 +154,52 @@ Global Instance galois_pairs :
   gamma_monotone := gamma_pairs_monotone;
 }.
 End galois_pairs.
-Hint Constructors gamma_pairs : soundness.
-
-(*
-Section galois_result.
-Context {A A': Type} `{Galois A' A}.
-
-Inductive gamma_result : abstract_result A abstract_store -> 
-                          result A' store -> Prop :=
-  fun r1 => fun r2 => match r1, r2 with
-                      | returnRA a s, returnR b t => 
-                          gamma a b /\ gamma s t
-                      | crashedA , _ => True
-                      | exceptionA st, exception st' => gamma st st'
-                      | exceptionOrReturn x st, exception st' =>
-                          gamma st st'
-                      | exceptionOrReturn x st, returnR x' st' =>
-                          gamma st st' /\ gamma x x'
-                      | _, _ => False
-                      end.
-
-Lemma gamma_result_monotone :
-  monotone gamma_result.
-Proof.
-  unfold monotone. intros a a' Hpred. simpl in *. constructor. 
-  intros x Hgamma.
-  inversion Hpred; subst.
-  - reflexivity.
-  - destruct x; try inversion Hgamma.
-    eapply widen. apply H1. apply Hgamma.
-  - destruct x; try inversion Hgamma.
-    split; eapply widen. apply H1. auto. apply H2. auto.
-  - destruct x; try inversion Hgamma.
-    eapply widen. apply H1. apply Hgamma.
-  - destruct x; try inversion Hgamma.
-    split; eapply widen. apply H1. apply H4. apply H2. apply H3.
-  - destruct x; try inversion Hgamma.
-    + split. eapply widen. apply H2. apply H3.
-      eapply widen. apply H1. apply H4.
-    + eapply widen. apply H2. apply Hgamma.
-Qed.
-
-Global Instance galois_result :
-  Galois (result A' store) (abstract_result A abstract_store) :=
-{
-  gamma := gamma_result;
-  gamma_monotone := gamma_result_monotone;
-}.
-
-End galois_result.
-*)
+Hint Unfold gamma_pairs : soundness.
 
 Section galois_maybe.
   Context {A A'} `{Galois A A'}.
 
-  Inductive gamma_maybeA_maybe : AbstractMaybe A' -> Maybe A -> Prop :=
-    | gamma_noneA : forall x, gamma_maybeA_maybe (NoneA) x
-    | gamma_justA_just : 
-        forall x y, gamma x y -> gamma_maybeA_maybe (JustA x) (Just y)
-    | gamma_justnoneA_justA :
-        forall x y, gamma x y -> gamma_maybeA_maybe (JustOrNoneA x) (Just y)
-    | gamma_justnoneA_noneA : 
-        forall x, gamma_maybeA_maybe (JustOrNoneA x) (None).
+  Definition gamma_maybeA (am : AbstractMaybe A') (m : Maybe A) : Prop :=
+    match am, m with
+    | NoneA, _ 
+    | JustOrNoneA _, None => True
+    | JustA x, Just y
+    | JustOrNoneA x, Just y => gamma x y
+    | _, _ => False
+    end.
+  Hint Unfold gamma_maybeA : soundness.
 
-  Inductive gamma_maybe_maybe : Maybe A' -> Maybe A -> Prop :=
-    | gamma_none : forall x, gamma_maybe_maybe None x
-    | gamma_just : forall a b,
-        gamma a b -> gamma_maybe_maybe (Just a) (Just b).
+  Definition gamma_maybe (m : Maybe A') (n : Maybe A) : Prop :=
+    match m, n with
+    | None, _ => True
+    | Just x, Just y => gamma x y
+    | _, _ => False
+    end.
+  Hint Unfold gamma_maybe : soundness.
 
-  Lemma gamma_maybe_monotone : monotone gamma_maybeA_maybe.
+  Lemma gamma_maybeA_monotone : monotone gamma_maybeA.
   Proof.
-    constructor. intros m Hm. destruct m.
-    - inversion Hm; subst.
-      + destruct a'.
-        * inversion H1.
-        * inversion H1.
-        * constructor.
-      + destruct a'.
-        * inversion H1; subst. constructor. apply widen with (f:=x).
-          assumption. assumption.
-        * constructor. inversion H1; subst. apply widen with (f:=x).
-          assumption. assumption.
-        * constructor.
-      + destruct a'.
-        * inversion H1.
-        * inversion H1; subst. constructor. apply widen with (f:=x).
-          assumption. assumption.
-        * constructor.
-  - inversion Hm; subst; inversion H1; constructor.
+    simple_solve; apply_widen.
   Qed.
 
-  Lemma gamma_maybe_maybe_monotone : monotone gamma_maybe_maybe.
+  Lemma gamma_maybe_monotone : monotone gamma_maybe.
   Proof.
-    constructor. intros m Hm. destruct a, a', m; try constructor;
-      inv Hm; inv H1; try assumption. eapply widen.
-      apply H5. assumption.
+    simple_solve; apply_widen.
   Qed.
 
   Global Instance galois_maybe_maybeA : Galois (Maybe A) (AbstractMaybe A') :=
   {
-    gamma := gamma_maybeA_maybe;
-    gamma_monotone := gamma_maybe_monotone;
+    gamma := gamma_maybeA;
+    gamma_monotone := gamma_maybeA_monotone;
   }.
 
   Global Instance galois_maybe_maybe : Galois (Maybe A) (Maybe A') :=
   {
-    gamma := gamma_maybe_maybe;
-    gamma_monotone := gamma_maybe_maybe_monotone;
+    gamma := gamma_maybe;
+    gamma_monotone := gamma_maybe_monotone;
   }.
 End galois_maybe.
-Hint Constructors gamma_maybeA_maybe gamma_maybe_maybe : soundness.
+Hint Unfold gamma_maybeA gamma_maybe : soundness.
 
 Section galois_state.
 Context {A A'} 
@@ -332,18 +212,11 @@ Proof.
 Defined.
 End galois_state.
 
-
 Section galois_unit.
-Inductive gamma_unit : 
-  unit -> unit -> Prop :=  
-    | gamma_unit_tt :  gamma_unit tt tt.
-
+  Definition gamma_unit (u v : unit) : Prop := True.
 
 Lemma gamma_unit_monotone : monotone gamma_unit.
-Proof.
-  unfold monotone.
-  intros. simpl. constructor. intros x. destruct a, a', x. reflexivity.
-Qed.
+Proof. simple_solve. Qed.
 
 Global Instance galois_unit : Galois unit unit := 
 {
@@ -351,6 +224,6 @@ Global Instance galois_unit : Galois unit unit :=
   gamma_monotone := gamma_unit_monotone;
 }. 
 End galois_unit.
-Hint Constructors gamma_unit : soundness.
+Hint Unfold gamma_unit : soundness.
 
 
