Instances/IsNat/Parity.v
@@ -1,15 +1,14 @@
+Require Export Base.
+Require Import Classes.Applicative.
 Require Import Classes.IsNat.
 Require Import Classes.Monad.
-Require Import Types.Parity.
-Require Import Types.AbstractBool.
+Require Import Coq.Arith.Arith.
+Require Import Instances.Monad.
+Require Import Instances.Monad.
 Require Import Language.Statements.
-Require Import Types.Result.
-Require Import Types.Stores.
+Require Import Types.AbstractBool.
+Require Import Types.Parity.
 Require Import Types.State.
-Require Import Instances.Monad.
-Require Import Types.Maps.
-Require Import Classes.Applicative.
-Require Import Instances.Monad.
 
 Definition ensure_par (v : avalue) : AbstractState parity :=
   match v with
@@ -17,12 +16,47 @@ Definition ensure_par (v : avalue) : AbstractState parity :=
   | _ => liftT (pure NoneA)
   end.
 
-Fixpoint extract_par (n : nat) : parity :=
-  match n with 
-  | 0 => par_even
-  | S 0 => par_odd
-  | S (S n) => extract_par n
-end.
+Definition extract_par (n : nat) : parity :=
+  if Nat.even n then par_even else par_odd.
+Hint Unfold extract_par : soundness.
+
+Lemma extract_S_n : forall n,
+  extract_par (S n) = parity_plus (extract_par n) par_odd.
+Proof. 
+  simple_solve. 
+  - destruct n. discriminate. rewrite Nat.even_spec in Heqb.
+    rewrite Nat.even_succ in Heqb0. rewrite Nat.odd_spec in Heqb0.
+    exfalso. apply Nat.Even_Odd_False with (x:=n);
+    assumption. 
+  - destruct n. simpl in Heqb0. discriminate. rewrite Nat.even_succ in Heqb0.
+    assert ((Nat.even n || Nat.odd n)%bool = true).
+    apply Nat.orb_even_odd. rewrite Heqb in H. rewrite Heqb0 in H.
+    simpl in H. discriminate.
+Qed.
+
+Lemma even_extract_pareven_equiv : forall n,
+  Nat.Even n <-> extract_par n = par_even.
+Proof. 
+  intros. split; intro H. 
+  - unfold extract_par. destruct (Nat.even n) eqn:H'. reflexivity.
+    rewrite <- Nat.even_spec in H. rewrite H in H'. discriminate.
+  - unfold extract_par in H. destruct (Nat.even n) eqn:H'.
+    rewrite Nat.even_spec in H'. assumption. discriminate.
+Qed.
+
+Lemma odd_extract_parodd_equiv : forall n, 
+  Nat.Odd n <-> extract_par n = par_odd.
+Proof. 
+  split; intro H.
+  - unfold extract_par. unmatch (Nat.even n).
+    + rewrite Nat.even_spec in Heqb. exfalso. apply Nat.Even_Odd_False with
+      (x:=n); assumption.
+    + reflexivity.
+  - unfold extract_par in H. unmatch (Nat.even n). discriminate.
+    apply Nat.odd_spec. unfold Nat.odd. rewrite Heqb. auto.
+Qed.
+Hint Rewrite <- even_extract_pareven_equiv odd_extract_parodd_equiv :
+  soundness.
 
 Definition extract_parM (n : nat) : AbstractState parity :=
   liftT (pure (extract_par n)).
