Classes/Joinable.v
@@ -1,3 +1,4 @@
+Require Export Base.
 Require Import Classes.PreorderedSet.
 
 Class Joinable (T : Type) `{PreorderedSet T} : Type :=
@@ -6,4 +7,5 @@ Class Joinable (T : Type) `{PreorderedSet T} : Type :=
   join_upper_bound_left: forall t t', preorder t (join_op t t');
   join_upper_bound_right: forall t t', preorder t' (join_op t t');
 }.
+Hint Resolve join_upper_bound_left join_upper_bound_right : soundness.
 
