Classes/PreorderedSet.v
@@ -1,11 +1,12 @@
-Require Import Coq.Classes.RelationClasses.
+Require Export Base.
 
 Class PreorderedSet (X : Type) : Type :=
 {
   preorder : X -> X -> Prop;
-  preorder_refl: Reflexive preorder;
-  preorder_trans: Transitive preorder;
+  preorder_refl: forall x, preorder x x;
+  preorder_trans: forall x y z, preorder x y -> preorder y z -> preorder x z;
 }.
+Hint Resolve preorder_refl preorder_trans : soundness.
 
 Arguments Build_PreorderedSet X {_ _ _}.
 
@@ -13,3 +14,10 @@ Definition monotone {A A'} `{PreorderedSet A, PreorderedSet A'} :
   (A -> A') -> Prop :=
   fun f => forall (a a': A), preorder a a' -> preorder (f a) (f a').
   
+Hint Unfold monotone : soundness.
+
+Ltac pre_trans :=
+  match goal with
+  | H : preorder ?a ?b, K : preorder ?b ?c  |- preorder ?a ?c =>
+      eapply preorder_trans; [apply H|assumption]
+  end.
