Instances/Joinable.v
@@ -1,11 +1,13 @@
+Require Import Classes.Applicative.
+Require Import Classes.Functor.
 Require Import Classes.Joinable.
 Require Import Classes.PreorderedSet.
 Require Import Coq.Logic.FunctionalExtensionality.
+Require Import Instances.Monad.
 Require Import Instances.Preorder.
 Require Import Language.Statements.
 Require Import Types.Result.
 Require Import Types.Stores.
-Require Import Instances.Monad.
 
 Definition abstract_store_join
   (ast1 ast2 : abstract_store) : abstract_store :=
@@ -13,32 +15,20 @@ Definition abstract_store_join
 
 Lemma abstract_store_join_comm : forall ast1 ast2,
   abstract_store_join ast1 ast2 = abstract_store_join ast2 ast1.
-Proof. 
-  intros. unfold abstract_store_join. apply functional_extensionality.
-  intros. reflexivity. 
-Qed.
+Proof. simple_solve. Qed.
 
 Lemma abstract_store_join_assoc : forall ast1 ast2 ast3,
   abstract_store_join ast1 (abstract_store_join ast2 ast3) =
   abstract_store_join (abstract_store_join ast1 ast2) ast3.
-Proof. 
-  intros. unfold abstract_store_join. apply functional_extensionality.
-  intros. reflexivity.
-Qed.
+Proof. simple_solve. Qed.
 
 Lemma abstract_store_join_upperbound_left :
     forall s s', preorder s (abstract_store_join s s').
-Proof.
-  simpl. unfold abstract_store_join. constructor.
-  intro x. constructor.
-Qed.
+Proof. simple_solve. Qed.
 
 Lemma abstract_store_join_upperbound_right : 
   forall s s', preorder s' (abstract_store_join s s').
-Proof.
-  simpl. unfold abstract_store_join. constructor.
-  intro x. constructor.
-Qed.
+Proof. simple_solve. Qed.
 
 Global Instance abstract_store_joinable : Joinable abstract_store := {
   join_op := abstract_store_join;
@@ -46,21 +36,17 @@ Global Instance abstract_store_joinable : Joinable abstract_store := {
   join_upper_bound_right := abstract_store_join_upperbound_right;
 }.
 
-
 Definition unit_join : unit -> unit -> unit :=
     fun _ _ => tt.
+Hint Unfold unit_join : soundness.
 
 Lemma unit_join_upperbound_left : forall (u u' : unit),
   preorder u (unit_join u u').
-Proof.
-  intros. destruct u, u'. unfold unit_join. apply preorder_refl.
-Qed.
+Proof. simple_solve. Qed.
 
 Lemma unit_join_upperbound_right : forall (u u' : unit),
   preorder u' (unit_join u u').
-Proof.
-  intros. destruct u, u'. unfold unit_join. apply preorder_refl.
-Qed.
+Proof. simple_solve. Qed.
 
 Global Instance unit_joinable : Joinable unit :=
 {
@@ -68,64 +54,6 @@ Global Instance unit_joinable : Joinable unit :=
   join_upper_bound_left := unit_join_upperbound_left;
   join_upper_bound_right := unit_join_upperbound_right
 }.
-
-
-Section result_joinable.
-Context {A S : Type} `{Joinable A, Joinable S}.
-
-Definition join_result (r1 r2 : abstract_result A S) : abstract_result A S :=
-  match r1, r2 with
-  | crashedA , _ | _, crashedA => crashedA 
-  | exceptionA s1, exceptionA s2 => exceptionA (join_op s1 s2)
-  | returnRA a1 s1, returnRA a2 s2 => returnRA (join_op a1 a2) (join_op s1 s2)
-  | exceptionA s1, returnRA a2 s2 => exceptionOrReturn a2 (join_op s1 s2)
-  | returnRA a1 s1, exceptionA s2 => exceptionOrReturn a1 (join_op s1 s2)
-  | exceptionOrReturn a1 s1, exceptionOrReturn a2 s2 =>
-      exceptionOrReturn (join_op a1 a2) (join_op s1 s2)
-  | _ , _ => crashedA 
-  end.
-
-Lemma join_result_upperbound_left :
-  forall r1 r2, preorder r1 (join_result r1 r2).
-Proof. 
-  intros r1 r2. simpl. destruct r1.
-  - destruct r2; simpl; constructor. simpl. 
-    apply join_upper_bound_left. apply join_upper_bound_left.
-    apply join_upper_bound_left. apply preorder_refl.
-  - simpl. constructor.
-  - simpl. destruct r2; simpl; try constructor.
-    apply join_upper_bound_left.
-    apply join_upper_bound_left.
-  - simpl. destruct r2; simpl; try constructor.
-    apply join_upper_bound_left.
-    apply join_upper_bound_left.
-Qed.
-
-Lemma join_result_upperbound_right :
-  forall r1 r2, preorder r2 (join_result r1 r2).
-Proof. 
-  intros r1 r2. simpl. destruct r1.
-  - destruct r2; simpl; constructor. simpl. 
-    apply join_upper_bound_right.
-    apply join_upper_bound_right.
-    apply join_upper_bound_right.
-  - simpl. constructor.
-  - simpl. destruct r2; simpl; constructor.
-    apply join_upper_bound_right.
-    apply preorder_refl.
-    apply join_upper_bound_right.
-  - simpl. destruct r2; simpl; try constructor.
-    apply join_upper_bound_right.
-    apply join_upper_bound_right.
-Qed.
-
-Global Instance result_joinable : Joinable (abstract_result A S) := {
-  join_op := join_result;
-  join_upper_bound_left := join_result_upperbound_left;
-  join_upper_bound_right := join_result_upperbound_right;
-}.
-
-End result_joinable.
 
 Section state_joinable.
   Context {S A} `{Joinable S, Joinable A}.
@@ -136,19 +64,11 @@ Section state_joinable.
   
   Lemma state_join_upper_bound_left :
     forall st st', preorder st (state_join st st').
-  Proof. 
-    intros. constructor. intros. unfold state_join.
-    destruct (st x), (st' x). constructor;
-    apply join_upper_bound_left. 
-  Qed.
+  Proof. simple_solve. Qed.
 
   Lemma state_join_upper_bound_right :
     forall st st', preorder st' (state_join st st').
-  Proof.
-    intros. constructor. intros. unfold state_join.
-    destruct (st x), (st' x). constructor;
-    apply join_upper_bound_right.
-  Qed.
+  Proof. simple_solve. Qed.
 
 Global Instance state_joinable : Joinable (State S A) := {
   join_op := state_join;
@@ -175,18 +95,15 @@ Definition join_maybe_abstract
                            JustOrNoneA (join_op x y)
                        end
   end.
+Hint Unfold join_maybe_abstract : soundness.
 
 Lemma join_maybe_abstract_upperbound_left : forall st st',
   preorder st (join_maybe_abstract st st').
-Proof.
-  intros. destruct st, st'; constructor; apply join_upper_bound_left.
-Qed.
+Proof. simple_solve. Qed.
 
 Lemma join_maybe_abstract_upperbound_right : forall st st',
   preorder st' (join_maybe_abstract st st').
-Proof.
-  intros. destruct st, st'; constructor; apply join_upper_bound_right.
-Qed.
+Proof. simple_solve. Qed.
 
 Global Instance abstract_maybe_joinable : Joinable (AbstractMaybe A) := 
 {
@@ -197,9 +114,6 @@ Global Instance abstract_maybe_joinable : Joinable (AbstractMaybe A) :=
 
 End abstract_maybe_joinable.
 
-  Require Import Classes.Applicative.
-  Require Import Classes.Functor.
-
 Section joinable_maybeAT.
   Context {A} `{Joinable A}.
   Context {M : Type -> Type} `{Monad M, 
@@ -207,6 +121,7 @@ Section joinable_maybeAT.
   
   Definition join_maybeAT : MaybeAT M A -> MaybeAT M A-> MaybeAT M A := 
     liftA2 join_op.
+  Hint Unfold join_maybeAT : soundness.
 
   Global Instance maybeAT_joinable : Joinable (MaybeAT M A) :=
   {
