Soundness.v
@@ -1,4 +1,5 @@
 Require Export Base.
+Require Export Instances.Galois.
 Require Import Classes.Galois.
 Require Import Classes.IsBool.
 Require Import Classes.IsNat.
@@ -9,13 +10,13 @@ Require Import Coq.Arith.Arith.
 Require Import Coq.Arith.Even.
 Require Import Coq.Arith.PeanoNat.
 Require Import Instances.Except.AbstractException.
-Require Export Instances.Galois.
 Require Import Instances.IsBool.AbstractBoolean.
 Require Import Instances.IsBool.Boolean.
+Require Import Instances.IsNat.Interval.
 Require Import Instances.IsNat.Nat.
 Require Import Instances.IsNat.Parity.
-Require Import Instances.IsNat.Interval.
 Require Import Instances.Joinable.
+Require Import Instances.Monad.
 Require Import Instances.Store.AbstractStore.
 Require Import Language.Statements.
 Require Import SharedInterpreter.
@@ -25,8 +26,6 @@ Require Import Types.Parity.
 Require Import Types.State.
 Require Import Types.Stores.
 
-
-Arguments gamma : simpl never.
 Arguments join_op : simpl never.
 
 Hint Extern 5 (gamma ?A ?B) => constructor : soundness.
@@ -42,18 +41,17 @@ Lemma gamma_fun_apply {A A' B B'} `{Galois A A', Galois B B'}
     (f : A -> B) (f' : A' -> B') x x' :
   gamma f' f -> gamma x' x ->
   gamma (f' x') (f x).
-Proof. Admitted.
-(*
-Proof. intros ??. constructor. apply H3. apply H4. Q *)
+Proof. eauto with soundness. Qed.
 Hint Resolve gamma_fun_apply : soundness.
-
 
 Lemma gamma_fun_applied {A A' B B'} `{Galois A A', Galois B B'}
     (f : A -> B) (f' : A' -> B') :
       (forall x x', gamma x' x -> gamma (f' x') (f x)) ->
         gamma f' f.
-Proof. constructor. intros. apply H3. apply H4. Qed.
-(*Hint Resolve gamma_fun_applied : soundness. *)
+Proof. 
+  intro. simpl; unfold gamma_fun. eauto with soundness. 
+Qed.
+Hint Resolve gamma_fun_applied : soundness.
 
 (*Require Import Instances.Monad.
 Lemma return_state_sound :
@@ -67,122 +65,137 @@ Qed.*)
 Lemma gamma_par_extract_n_n : forall n,
   gamma (extract_par n) n.
 Proof.
-  intros. pose proof even_or_odd as Hpar. 
-  destruct Hpar with (n:=n) as [Heven | Hodd].
-  - rewrite even_extract_pareven; try constructor; assumption.
-  - rewrite odd_extract_parodd; try constructor; assumption.
+  intros. autounfold with soundness. simpl. autounfold with soundness.
+  destruct (Nat.even n) eqn:Hpar. 
+  - rewrite Nat.even_spec in Hpar. assumption.
+  - pose proof Nat.negb_even. 
+    rewrite <- Nat.odd_spec. rewrite <- Nat.negb_even, Bool.negb_true_iff.
+    assumption.
 Qed.
 Hint Resolve gamma_par_extract_n_n : soundness.
 
 Lemma parity_plus_sound :
   gamma parity_plus plus.
-Proof. repeat constructor. intros a' b' H'.  
-  destruct a, a'; inversion H; subst; inversion H';
-  subst; constructor;
-  auto using even_even_plus, odd_plus_r, odd_plus_l, odd_even_plus.
+Proof.
+  apply gamma_fun_applied. intros. apply gamma_fun_applied. intros.
+  unfold parity_plus. destruct x', x'0; simple_solve.
 Qed.
 Hint Resolve parity_plus_sound : soundness.
 
 Lemma parity_mult_sound :
   gamma parity_mult mult.
-Proof. repeat constructor. intros a0 b0 H0. destruct a, a0; 
-  inversion H; subst; inversion H0; subst;
-  simpl in *; try tauto; 
-  constructor; auto using even_mult_l, even_mult_r, odd_mult.
+Proof. 
+  simple_solve.
 Qed.
 Hint Resolve parity_mult_sound : soundness.
 
+Hint Rewrite Nat.eqb_eq : soundness.
 Lemma parity_eq_sound :
   gamma parity_eq Nat.eqb. 
-Proof. repeat constructor. intros a0 b0 H0.
-  destruct a, a0; inversion H; inversion H0; subst; try constructor.
-  - assert ((b =? b0) = false) as contra. 
-    apply Nat.eqb_neq. unfold not. intros; subst. eauto using not_even_and_odd.
-    rewrite contra. simpl. apply gamma_false. 
-  - assert (b =? b0 = false) as contra. 
-    apply Nat.eqb_neq. unfold not. intros; subst. 
-    eauto using not_even_and_odd. rewrite contra. simpl. apply gamma_false.
+Proof. 
+  simple_solve.
 Qed.
 Hint Resolve parity_eq_sound : soundness.
 
 Lemma extract_par_sound : forall n,
   gamma (VParity (extract_par n)) (VNat n).
-Proof. auto with soundness. Qed.
+Proof. 
+  simple_solve. rewrite Nat.even_spec in Heqb. assumption.
+  rewrite <- Nat.odd_spec. unfold Nat.odd. rewrite Heqb.
+  reflexivity.
+Qed.
 
+Lemma lift_maybeAT_sound : gamma lift_maybeAT lift_maybeT.
+Proof.
+Admitted.
 (* Monadic versions of parity operations *)
-
+Hint Unfold gamma : soundness.
 Lemma ensure_par_sound : 
   gamma ensure_par ensure_nat.
 Proof.
-  repeat constructor. intros.
-  destruct a.
-  - gamma_destruct. unfold ensure_par, ensure_nat. 
-    unfold gamma. simpl. unfold gamma_maybe_maybe.
-
-    repeat constructor; gamma_destruct; try assumption.
-  - gamma_destruct; repeat constructor; assumption.
-  - gamma_destruct; repeat constructor; assumption.
-  - gamma_destruct; repeat constructor; try assumption. 
-    unfold ensure_par, ensure_nat. destr; repeat constructor; assumption.
-  - gamma_destruct.
-Qed.
+  (*simpl; unfold gamma_fun; intros.
+  simpl; unfold gamma_fun; intros.
+  simpl; unfold gamma_maybe. destruct (ensure_par a a0) eqn:?; try reflexivity.
+  destruct (ensure_nat b b0) eqn:?.
+  - simpl in *. unfold gamma_pairs. destruct p eqn:?. destruct p0 eqn:?.
+  - simpl in H, H0. unfold ensure_par in Heqm. unfold liftT in Heqm.
+    simpl in Heqm.*)
+Admitted.
+  
 Hint Resolve ensure_par_sound : soundness.
 
 Lemma extract_parM_sound :  forall n,
   gamma (extract_parM n) (extract_natM n). 
-Proof. repeat constructor; simpl; destruct H;
+Proof. 
+  (*simpl. unfold gamma_fun. simpl. intros. unfold extract_parM, extract_natM.
+  simple_solve.
+  repeat constructor; simpl; destruct H;
   auto with soundness. destruct H0. apply H0.
-Qed.
+*)
+Admitted.
 Hint Resolve extract_parM_sound : soundness.
 
 Lemma pplusM_sound : 
   gamma pplusM plusM.
 Proof. 
-  repeat constructor; simpl; eauto with soundness.
+  simpl; unfold gamma_fun; intros.
+  simpl; unfold gamma_fun; intros.
+  simpl; unfold gamma_fun; intros.
+  unfold pplusM, plusM. 
+Admitted.
+(*  repeat constructor; simpl; eauto with soundness.
+
   destruct H2. apply H2. destruct H1. apply H1.
-Qed.
+Qed.*)
 Hint Resolve pplusM_sound : soundness.
 
 Lemma pmultM_sound :
   gamma pmultM multM.
 Proof.
-  repeat constructor; simpl; eauto with soundness. 
+  (*repeat constructor; simpl; eauto with soundness. 
   destruct H2; assumption.
-  destruct H1; assumption.
-Qed.
+  destruct H1; assumption.*)
+Admitted.
 Hint Resolve pmultM_sound : soundness.
 
 Lemma peqM_sound :
   gamma peqM eqbM.
 Proof.
+  (*
   repeat constructor; simpl. eauto with soundness.
   destruct H2; assumption.
   destruct H1; assumption.
-Qed.
+*)
+Admitted.
 Hint Resolve peqM_sound : soundness.
 
 Lemma pleM_sound :
   gamma pleM lebM.
 Proof.
+  (*
   repeat constructor; simpl; eauto with soundness.
   destruct H2; assumption.
   destruct H1; assumption.
-Qed.
+*)
+Admitted.
 Hint Resolve pleM_sound : soundness.
 
 Lemma build_parity_sound :
   gamma build_parity build_natural.
 Proof.
+(*
   repeat constructor. assumption. 
   destruct H1; assumption.
   destruct H0; assumption.
-Qed.
+*)
+Admitted.
 Hint Resolve build_parity_sound : soundness.
 
 (* Soundness of operations on intervals *)
 Lemma iplusM_sound :
   gamma iplusM plusM.
 Proof. 
+(*
   repeat constructor; simpl; destruct H, H0.
   rewrite Interval.interval_min_plus;
   apply Coq.Arith.Plus.plus_le_compat; assumption.
@@ -190,12 +203,14 @@ Proof.
   apply Coq.Arith.Plus.plus_le_compat; assumption.
   destruct H2; assumption.
   destruct H1; assumption.
-Qed.
+*)
+Admitted.
 Hint Resolve iplusM_sound : soundness.
 
 Lemma imultM_sound :
   gamma imultM multM.
 Proof.
+  (*
   repeat constructor; simpl; destruct H, H0.
   rewrite Interval.interval_min_mult;
   apply Coq.Arith.Mult.mult_le_compat; assumption.
@@ -203,12 +218,14 @@ Proof.
   apply Coq.Arith.Mult.mult_le_compat; assumption.
   destruct H2; assumption.
   destruct H1; assumption.
-Qed.
+*)
+Admitted.
 Hint Resolve imultM_sound.
 
 Lemma ileqb_sound :
   gamma ileM lebM.
 Proof.
+  (*
   repeat constructor; simpl. destruct H, H0. destruct i, i0. simpl in *.
   unfold Interval.ileqb.
   destruct (Interval.max (n1, n2) <? Interval.min (n3, n4)) eqn:Hint.
@@ -231,11 +248,13 @@ Proof.
     + constructor. 
   - destruct H2; assumption.
   - destruct H1; assumption.
-Qed.
+    *)
+  Admitted.
 Hint Resolve ileqb_sound : soundness.
 
 Lemma ieqM_sound : gamma ieqM eqbM.
 Proof.
+  (*
   repeat constructor. simpl. destruct H, H0. 
   unfold Interval.ieqb. 
   destruct (Interval.max i <? Interval.min i0) eqn:Hdiff.
@@ -254,36 +273,43 @@ Proof.
   - destruct H2; assumption.
   - destruct H1; assumption.
 Qed.
+*)
+Admitted.
 Hint Resolve ieqM_sound : soundness.
 
 Lemma build_interval_sound :
   gamma build_interval build_natural.
 Proof.
+  (*
   repeat constructor; destruct H; try assumption.
   destruct H1; assumption.
   destruct H0; assumption.
-Qed.
+*)
+Admitted.
 Hint Resolve build_interval_sound : soundness.
 
 Lemma extract_interval_sound : forall n,
   gamma (extract_interval n) (extract_natM n).
 Proof.
-  intros n. repeat constructor. 
+  (*intros n. repeat constructor. 
   simpl. rewrite Interval.interval_min_refl. reflexivity. 
   rewrite Interval.interval_max_refl. reflexivity.
   destruct H0; assumption.
   destruct H; assumption.
-Qed.
+*)
+Admitted.
 Hint Resolve extract_interval_sound : soundness.
 
 Lemma ensure_interval_sound : gamma ensure_interval ensure_nat.
 Proof.
+  (*
   repeat constructor. intros. destruct a;
   inv H; repeat constructor. destruct H0; assumption. destruct H0; assumption.
   destruct H2; assumption. destruct H2; assumption. destruct H; assumption.
   destruct H0; assumption. destruct b; repeat constructor; destruct H0;
   assumption.
-Qed.
+*)
+Admitted.
 Hint Resolve ensure_interval_sound : soundness.
 
 (* Soundness of operations on booleans *)
@@ -291,33 +317,45 @@ Hint Resolve ensure_interval_sound : soundness.
 Lemma ab_and_sound :
   gamma and_ab andb.
 Proof. 
+  (*
   repeat constructor. intros. 
   destruct b, b0, a, a0; try constructor; try inv H; try inv H0.
-Qed.
+*)
+Admitted.
 
 Lemma ab_or_sound :
   gamma or_ab orb.
-Proof. repeat constructor; intros.
+Proof. 
+  (*
+  repeat constructor; intros.
   destruct b, b0, a, a0; try constructor; try inv H; try inv H0.
-Qed.
+*)
+Admitted.
 Hint Resolve ab_or_sound : soundness.
 
 Lemma ab_neg_sound :
   gamma neg_ab negb.
-Proof. repeat constructor. intros ? ? ?. 
+Proof. 
+  (*
+  repeat constructor. intros ? ? ?. 
   destruct a, b; try constructor; try inversion H.
-Qed.
+*)
+Admitted.
 
 Lemma extract_bool_sound : forall x,
   gamma (VAbstrBool (extract_ab x)) (VBool x).
-Proof. repeat constructor. destruct x; constructor. Qed.
+Proof. 
+  (*repeat constructor. destruct x; constructor. *)
+Admitted.
 Hint Resolve extract_bool_sound : soundness.
 
 (* Monadic operations on abstract booleans *)
 
 Lemma ensure_abool_sound :
   gamma ensure_abool ensure_bool.
-Proof. repeat constructor. intros.
+Proof. 
+  (*
+  repeat constructor. intros.
   destruct a; try constructor. destruct b; try inv H.
   repeat constructor. destruct H0; assumption. 
   inv H. repeat constructor. assumption. inv H; assumption.
@@ -326,41 +364,44 @@ Proof. repeat constructor. intros.
   constructor. assumption. constructor. assumption. destruct b.
   constructor. constructor. assumption. constructor. constructor.
   assumption.
-Qed.
+*)
+Admitted.
 Hint Resolve ensure_abool_sound : soundness.
 
 Lemma neg_abM_sound :
   gamma neg_abM negbM.
 Proof.
+  (*
   repeat constructor; simpl. apply gamma_fun_apply.
   apply ab_neg_sound. assumption. 
   inv H1; assumption. inv H0; assumption.
-Qed.
+*)
+Admitted.
 Hint Resolve neg_abM_sound : soundness.
 
 Lemma and_abM_sound :
   gamma and_abM andbM.
 Proof.
-  repeat constructor; simpl. repeat apply gamma_fun_apply.
+  (*repeat constructor; simpl. repeat apply gamma_fun_apply.
   apply ab_and_sound. assumption. assumption. inv H2; assumption.
-  inv H1; assumption.
-Qed.
+  inv H1; assumption.*)
+Admitted.
 Hint Resolve and_abM_sound : soundness.
 
 Lemma extract_abM_sound: forall b,
   gamma (extract_abM b) (extract_boolean b).
 Proof. 
-  repeat constructor; simpl. destruct b; constructor.
-  inv H0; assumption. inv H; assumption.
-Qed.
+  (*repeat constructor; simpl. destruct b; constructor.
+  inv H0; assumption. inv H; assumption.*)
+Admitted.
 Hint Resolve extract_abM_sound : soundness.
 
 Lemma build_boolean_sound :
   gamma build_abool build_bool.
 Proof.
-  repeat constructor. assumption. inv H1; assumption.
-  inv H0; assumption.
-Qed.
+  (*repeat constructor. assumption. inv H1; assumption.
+  inv H0; assumption.*)
+Admitted.
 Hint Resolve build_boolean_sound : soundness.
 
 (* Soundness of applied functions *)
@@ -374,13 +415,13 @@ Hint Resolve functions_sound : soundness.*)
 
 (* Soundness of operations on stores *)
 
-Lemma store_get_sound : forall s,
+(*Lemma store_get_sound : forall s,
   gamma (abstract_store_get s) (store_get s).
 Proof.
   repeat constructor. inv H0. apply H1. inv H0; assumption.
   inv H; assumption.
 Qed.
-Hint Resolve store_get_sound : soundness.
+Hint Resolve store_get_sound : soundness.*)
 
 Lemma t_update_sound : forall (ast : abstract_store) (st : store) x p n,
   gamma ast st ->
@@ -388,11 +429,11 @@ Lemma t_update_sound : forall (ast : abstract_store) (st : store) x p n,
   gamma (t_update ast x p) (t_update st x n).
 Proof. 
   repeat constructor.
-  unfold t_update. intro x'.
-  destruct (beq_string x x'); auto. destruct H. apply H.
+  unfold t_update. intros. simpl. unfold gamma_store. intro x'.
+  destruct (beq_string x x'); auto. 
 Qed.
 
-Lemma store_put_sound : forall s,
+(*Lemma store_put_sound : forall s,
   gamma (abstract_store_put s) (store_put s).
 Proof. 
   repeat constructor; simpl.
@@ -400,9 +441,9 @@ Proof.
   inv H1. apply H2. inv H0; assumption.
 Qed.
 Hint Resolve store_put_sound : soundness.
+*)
 
 (* Soundness of states *)
-Require Import Instances.Monad.
 Lemma bind_state_sound {S S' A A' B B'} 
   `{Galois S S'}
   `{Galois A A', Galois B B'} : 
@@ -412,12 +453,10 @@ Lemma bind_state_sound {S S' A A' B B'}
   gamma (@bind_state S' A' B' f' k') (@bind_state S A B f k).
 Proof.
   unfold bind_state. repeat constructor. intros.
+  simpl; unfold gamma_fun; intros.
+  apply H5 in H7.
   destruct (f' a) eqn:Hfa, (f b) eqn:Hfb.
-  inv H5.
-  destruct (k' a0 s) eqn:Hk', (k a1 s0) eqn:Hk.
-  inv H6. apply H8 in H7. rewrite Hfa, Hfb in H7. inv H7.
-  apply H5 in H11. inv H11. apply H6 in H13. rewrite Hk', Hk in H13.
-  apply H13.
+  apply H6; apply H7.
 Qed.
 Hint Resolve bind_state_sound : soundness.
 (*
@@ -444,16 +483,31 @@ Lemma extract_build_val_sound : forall v,
         (extract_build_val (M:=ConcreteState) v).
 Proof.
   destruct v; simpl; eauto with soundness.
-Qed.
+Admitted.
 Hint Resolve extract_build_val_sound : soundness.
+
+
+Require Import Classes.Store.
+Require Import Stores.
+Instance conc_store : Store store ConcreteState cvalue.
+Admitted.
+Instance abs_store : Store abstract_store AbstractState avalue.
+Admitted.
 
 Theorem eval_expr_sound : forall a,
   gamma (shared_eval_expr (M:=AbstractState) (A:=isnat_parity) a) 
-        (shared_eval_expr (M:=State) a).
+        (shared_eval_expr (M:=ConcreteState) a).
 Proof.
-  intros. induction a; simpl;
-  eauto 30 with soundness. 
-Qed.
+  intros. induction a; simpl.
+  - eauto with soundness.
+  - eauto with soundness. admit.
+  - eauto with soundness. admit.
+  - eauto with soundness. admit.
+  - eauto with soundness. admit.
+  - eauto with soundness. admit.
+  - eauto with soundness. admit.
+  - eauto with soundness. admit.
+Admitted.
 Hint Resolve eval_expr_sound : soundness.
 
 Lemma sound_if_op : 
@@ -461,22 +515,22 @@ Lemma sound_if_op :
   (eval_if).
 Proof.
   intros ????????????. 
-  destruct b; simpl. 
+  destruct b. 
   - (* true *)
-    destruct a; simpl. 
+    destruct a. 
     + apply H0. apply H2.
-    + unfold gamma in H; simpl in H. tauto.
-    + eapply widen. apply join_upper_bound_left. apply H0. apply H2.
-    + unfold gamma in H; simpl in H. tauto.
+    + unfold gamma in H; simpl in H. contradiction.
+    + unfold eval_if_abstract, eval_if. admit.
+    + unfold gamma in H; simpl in H. contradiction.
   - destruct a; simpl.
-    + unfold gamma in H; simpl in H; tauto.
+    + unfold gamma in H; simpl in H; contradiction.
     + apply H1. apply H2.
-    + eapply widen. apply join_upper_bound_right. apply H1. apply H2.
-    + unfold gamma in H; simpl in H; tauto.
-Qed.
+    + apply H1. apply H2.
+    + unfold gamma in H; simpl in H; contradiction.
+Admitted.
 Hint Resolve sound_if_op : soundness.
 
-Lemma sound_eval_catch :
+(*Lemma sound_eval_catch :
   gamma (eval_catch_abstract) (eval_catch).
 Proof.
   intros s1' s1 H s2' s2. intros H0 a b H1. 
@@ -502,21 +556,26 @@ Proof.
       pose proof H1. apply H0 in H1.  apply H1.
 Qed.
 Hint Resolve sound_eval_catch : soundness.
-
+*)
+  (*
 Lemma sound_fail : 
   gamma fail_abstract fail.
 Proof.
   unfold fail_abstract, fail. intros ???. auto.
 Qed.
 Hint Resolve sound_fail : soundness.
+*)
+
+Require Import Classes.Except.
+Instance except_conc : Except ConcreteState. Admitted.
 
 Theorem sound_interpreter:
   forall c, gamma (shared_ceval 
                     (M:=AbstractState) 
                     (A:=isnat_parity)
                     c) 
-                  (shared_ceval c).
+                  (shared_ceval (M:=ConcreteState) c).
 Proof.
-  induction c; simpl; eauto 30 with soundness.
-Qed.
+  induction c; simpl. eauto with soundness.
+Admitted.
 
