Types/Parity.v
@@ -1,8 +1,8 @@
+Require Export Base.
 Require Import Coq.Arith.Arith.
 Require Import Coq.Arith.PeanoNat.
 Require Import Coq.Arith.Even.
 Require Import Coq.Sets.Partial_Order.
-
 Require Import Types.AbstractBool.
 
 (** * Parity *)
@@ -34,17 +34,16 @@ Definition parity_plus (p q : parity) : parity :=
                end
   | par_bottom => par_bottom
   end.
+Hint Unfold parity_plus : soundness.
 
 Lemma parity_plus_par_even : forall p,
-  p = parity_plus p par_even.
-Proof.
-  destruct p; reflexivity.
-Qed.
+  parity_plus p par_even = p.
+Proof. intros. destruct p; reflexivity. Qed.
 
 Corollary parity_plus_par_odd : forall p,
   parity_plus p par_odd = par_even -> p = par_odd.
-Proof. 
-  intros. destruct p; try reflexivity; try inversion H.
+Proof.
+  intros; destruct p; try inv H; reflexivity.
 Qed.
 
 Lemma parity_plus_assoc : forall p q r,
@@ -66,7 +65,7 @@ Definition parity_mult (p q : parity) : parity :=
   | par_top => par_top
   | par_bottom => par_bottom
   end.
-
+Hint Unfold parity_mult : soundness.
 
 (** Equality *)
 Definition parity_eq (p1 p2 : parity) : abstr_bool :=
@@ -85,3 +84,49 @@ Definition parity_leb (p1 p2 : parity) : abstr_bool :=
   | par_even, par_even | par_odd, par_odd => ab_top
   | par_top, _ | _, par_bottom => ab_false
   end.
+
+(* Some lemmas regarding Nat.Even and Nat.Odd that are missing but are included
+ * for the deprecated even and odd. We define these lemmas here so we can use the  * newer definitions for when the older version are deleted. *)
+Lemma Even_add : forall n m, Nat.Even n -> Nat.Even m -> Nat.Even (n + m).
+Proof.
+  intros. rewrite <- Nat.even_spec in *. 
+  replace true with (Bool.eqb (Nat.even n) (Nat.even m)).
+  apply Nat.even_add. rewrite H, H0. reflexivity.
+Qed.
+
+Lemma Odd_Odd_add : forall n m, Nat.Odd n -> Nat.Odd m -> Nat.Even (n + m).
+Proof.
+  intros. rewrite <- even_equiv. 
+  rewrite <- odd_equiv in H, H0. apply odd_even_plus; assumption.
+Qed.
+
+Lemma Odd_Even_add : forall n m, Nat.Odd n -> Nat.Even m -> Nat.Odd (n + m).
+Proof.
+  intros. rewrite <- even_equiv in H0. rewrite <- odd_equiv in H.
+  rewrite <- odd_equiv. apply odd_plus_l; assumption.
+Qed.
+
+Lemma Even_Odd_add : forall n m, Nat.Even n -> Nat.Odd m -> Nat.Odd (n + m).
+Proof.
+  intros. rewrite <- even_equiv in H. rewrite <- odd_equiv in H0.
+  rewrite <- odd_equiv. apply odd_plus_r; assumption.
+Qed.
+
+Lemma Even_mult_l : forall n m, Nat.Even n -> Nat.Even (n * m).
+Proof.
+  intros. rewrite <- even_equiv in *. apply even_mult_l. assumption.
+Qed.
+
+Lemma Even_mult_r : forall n m, Nat.Even m -> Nat.Even (n * m).
+Proof.
+  intros. rewrite <- even_equiv in *. apply even_mult_r; assumption.
+Qed.
+
+Lemma Odd_mult : forall n m, Nat.Odd n -> Nat.Odd m -> Nat.Odd (n * m).
+Proof.
+  intros. rewrite <- odd_equiv in *. apply odd_mult; assumption.
+Qed.
+
+Hint Resolve Even_add Odd_Odd_add Odd_Even_add Even_Odd_add : soundness.
+Hint Resolve Even_mult_l Even_mult_r Odd_mult : soundness.
+Hint Resolve Nat.Even_Odd_False : soundness. 
